progress in proofs

src/locomp.lean
@@ -1,12 +1,22 @@
-import .love08_operational_semantics_demo .love01_definitions_and_statements_demo
+-- import .love08_operational_semantics_demo .love01_definitions_and_statements_demo
+import data.real.basic
+import data.vector
+import tactic.explode
+import tactic.find
+import tactic.induction
+import tactic.linarith
+import tactic.rcases
+import tactic.rewrite
+import tactic.ring_exp
+import tactic.tidy
+import tactic.split_ifs
 
 
--- set_option pp.beta true
--- set_option pp.generalized_field_notation false
+set_option pp.beta true
+set_option pp.generalized_field_notation false
 
 namespace LoComp
 
-open LoVe
 
 def vname := string
 
@@ -14,7 +24,164 @@ def val := ℤ
 
 def stack := list ℤ -- TODO: ???val??? how do we make it accept, because +, -, *, / is not defined for val
 
-def state := vname → ℤ
+
+namespace rtc
+
+inductive star {α : Sort*} (r : α → α → Prop) (a : α) : α → Prop
+| refl {}    : star a
+| tail {b c} : star b → r b c → star c
+
+attribute [refl] star.refl
+
+namespace star
+
+variables {α : Sort*} {r : α → α → Prop} {a b c d : α}
+
+@[trans] lemma trans (hab : star r a b) (hbc : star r b c) :
+  star r a c :=
+begin
+  induction' hbc,
+  case refl {
+    assumption },
+  case tail : c d hbc hcd hac {
+    exact (tail (hac hab)) hcd }
+end
+
+lemma single (hab : r a b) :
+  star r a b :=
+refl.tail hab
+
+lemma head (hab : r a b) (hbc : star r b c) :
+  star r a c :=
+begin
+  induction' hbc,
+  case refl {
+    exact (tail refl) hab },
+  case tail : c d hbc hcd hac {
+    exact (tail (hac hab)) hcd }
+end
+
+lemma head_induction_on {α : Sort*} {r : α → α → Prop} {b : α}
+  {P : ∀a : α, star r a b → Prop} {a : α} (h : star r a b)
+  (refl : P b refl)
+  (head : ∀{a c} (h' : r a c) (h : star r c b), P c h → P a (h.head h')) :
+  P a h :=
+begin
+  induction' h,
+  case refl {
+    exact refl },
+  case tail : b c hab hbc ih {
+    apply ih,
+    show P b _, from
+      head hbc _ refl,
+    show ∀a a', r a a' → star r a' b → P a' _ → P a _, from
+      assume a a' hab hbc, head hab _ }
+end
+
+lemma trans_induction_on {α : Sort*} {r : α → α → Prop}
+    {p : ∀{a b : α}, star r a b → Prop} {a b : α} (h : star r a b)
+    (ih₁ : ∀a, @p a a refl) (ih₂ : ∀{a b} (h : r a b), p (single h))
+    (ih₃ : ∀{a b c} (h₁ : star r a b) (h₂ : star r b c), p h₁ →
+       p h₂ → p (h₁.trans h₂)) :
+  p h :=
+begin
+  induction' h,
+  case refl {
+    exact ih₁ a },
+  case tail : b c hab hbc ih {
+    exact ih₃ hab (single hbc) (ih ih₁ @ih₂ @ih₃) (ih₂ hbc) }
+end
+
+lemma lift {β : Sort*} {s : β → β → Prop} (f : α → β)
+  (h : ∀a b, r a b → s (f a) (f b)) (hab : star r a b) :
+  star s (f a) (f b) :=
+hab.trans_induction_on
+  (assume a, refl)
+  (assume a b, single ∘ h _ _)
+  (assume a b c _ _, trans)
+
+lemma mono {p : α → α → Prop} :
+  (∀a b, r a b → p a b) → star r a b → star p a b :=
+lift id
+
+lemma star_star_eq :
+  star (star r) = star r :=
+funext
+  (assume a,
+   funext
+     (assume b,
+      propext (iff.intro
+        (assume h,
+         begin
+           induction' h,
+           { refl },
+           { transitivity;
+               assumption }
+         end)
+        (star.mono (assume a b,
+           single)))))
+
+end star
+
+end rtc
+
+export rtc
+
+
+def state : Type := vname → ℤ
+
+def state.update (name : vname) (val : ℤ) (s : state) : state :=
+λname', if name' = name then val else s name'
+
+notation s `{` name ` ↦ ` val `}` := state.update name val s
+
+instance : has_emptyc state :=
+{ emptyc := λ_, 0 }
+
+@[simp] lemma update_apply (name : vname) (val : ℤ) (s : state) :
+  s{name ↦ val} name = val :=
+if_pos rfl
+
+@[simp] lemma update_apply_ne (name name' : vname) (val : ℤ) (s : state)
+    (h : name' ≠ name) :
+  s{name ↦ val} name' = s name' :=
+if_neg h
+
+@[simp] lemma update_override (name : vname) (val₁ val₂ : ℤ) (s : state) :
+  s{name ↦ val₂}{name ↦ val₁} = s{name ↦ val₁} :=
+begin
+  apply funext,
+  intro name',
+  by_cases name' = name;
+    simp [h]
+end
+
+@[simp] lemma update_swap (name₁ name₂ : vname) (val₁ val₂ : ℤ) (s : state)
+    (h : name₁ ≠ name₂) :
+  s{name₂ ↦ val₂}{name₁ ↦ val₁} = s{name₁ ↦ val₁}{name₂ ↦ val₂} :=
+begin
+  apply funext,
+  intro name',
+  by_cases name' = name₁;
+    by_cases name' = name₂;
+    simp * at *
+end
+
+@[simp] lemma update_id (name : vname) (s : state) :
+  s{name ↦ s name} = s :=
+begin
+  apply funext,
+  intro name',
+  by_cases name' = name;
+    simp * at *
+end
+
+@[simp] lemma update_same_const (name : vname) (val : ℤ) :
+  (λ_, val){name ↦ val} = (λ_, val) :=
+by apply funext; simp
+
+
+
 
 def config := ℤ × state × stack
 
@@ -35,6 +202,7 @@ inductive instr : Type  -- page 35
 | JMP : int → instr
 | JMPLESS : int → instr
 | JMPGE : int → instr
+| NOP : instr           -- this is added to avoid option 
 
 
 open instr
@@ -48,7 +216,7 @@ def iexec : instr → config → config -- TODO: fill in the full matching
 | SUB (i, s, stk) := (i + 1, s, (head2 stk - stk.head) :: tail2 stk)
 | MUL (i, s, stk) := (i + 1, s, (head2 stk * stk.head) :: tail2 stk)
 | DIV (i, s, stk) := (i + 1, s, (head2 stk / stk.head) :: tail2 stk)
-| (STORE v) (i, s, stk) := (i + 1, s{v ↦ (stk.head)}, stk.tail) -- so state.update only works on the state that is not the correct one 
+| (STORE v) (i, s, stk) := (i + 1, s{v ↦ (stk.head)}, stk.tail)
 | (JMP n) (i, s, stk) := (i + 1 + n, s, stk)
 | (JMPLESS n) (i, s, stk) := 
   if (head2 stk) < (stk.head)
@@ -58,27 +226,61 @@ def iexec : instr → config → config -- TODO: fill in the full matching
   if (head2 stk) ≥ (stk.head)
   then (i + 1 + n, s, tail2 stk)
   else (i + 1, s, tail2 stk)
+| NOP (i, s, stk) := (i + 1, s, stk)
 
 /- redefinition for ints rather than nat -/ 
-def nth : list instr → ℤ → option instr  
-| (a :: l) 0 := option.some a
+def nth : list instr → ℤ → instr  
+| (a :: l) 0 := a
 | (a :: l) n := nth l (n - 1)
-| list.nil n := option.none
+| list.nil n := NOP
 
 
 /- 
   Execute one instruction
   check if pc is in a valid location in the list 
 -/
-def exec1  (li : list instr) (c : config)  (c' : config) : Prop := -- TODO: fix option/instr
-∃ i s stk, c = (i, s, stk) ∧ c' = iexec (nth li i) (i, s, stk) ∧ 0 ≤ i ∧ i < li.length  
+def exec1  (li : list instr) (c : config)  (c' : config) : Prop := 
+(∃ i s stk, c = (i, s, stk) ∧ c' = iexec (nth li i) (i, s, stk) ∧ 0 ≤ i ∧ i < li.length)  
 
 /-
 lemma exec1I [intro, code_pred_intro]:
   "c' = iexec (P!!i) (i,s,stk) ⟹ 0 ≤ i ⟹ i < size P
   ⟹ P ⊢ (i,s,stk) → c'"
 by (simp add: exec1_def)
+
 -/
+
+lemma exec1I {li : list instr} {i s stk c'}
+  (h1: c' = iexec (nth li i) (i, s, stk))
+  (h2 : 0 ≤ i) 
+  (h3 : i < li.length):
+  exec1 li (i, s, stk) c' := 
+  begin 
+    simp [exec1],
+    use i,
+    use s,
+    use stk,
+    simp [h1, h2, h3]
+  end
+
+lemma exec_trans {li : list instr} {c1 c2 c3 : config}
+  (h1 : exec1 li c1 c2)
+  (h2 : exec1 li c2 c3) :
+  exec1 li c1 c3 :=
+  begin
+    -- Use the definition of exec1 to unpack the assumptions
+    rcases h1 with ⟨i1, s1, stk1, hc1, hc2, hi1⟩,
+    rcases h2 with ⟨i2, s2, stk2, hc2', hc3, hi2⟩,
+    -- Use transitivity of execution to relate the two configurations
+    subst hc2,
+    have h : i1 < li.length,
+    { linarith [hi1, hi2] },
+    -- Apply exec1I lemma to obtain the transitivity lemma
+    exact exec1I hc3 hi1.left h,
+    -- TODO: replace exec1 right side of c3 with h1 items 
+  end
+
+
 
 
 abbreviation exec (li : list instr) (c : config) (c' : config) : Prop :=
@@ -97,6 +299,343 @@ lemma iexec_shift [simp]:
 by(auto split:instr.split)
 -/
 
+
+/-
+  if instruction is JMP/JMPLESS/JMPGE then it will have the next 
+  instruction pointer which is included in the shift
+-/
+lemma iexec_shift_with_jmp {n : ℤ}  {i' : ℤ} {i : ℤ} {instr : ℤ}:
+n + i' = n + i + 1 + instr ↔ i' = i + 1 + instr :=
+begin
+  apply iff.intro,
+  {
+    intro h_no_brackets,
+    have h_brackets: n + i' = n + (i + 1 + instr) := 
+    begin
+      simp [h_no_brackets],
+      cc,
+    end,
+    apply int.add_left_cancel,
+    apply h_brackets,
+  },
+  {
+    intro h3,
+    simp [h3],
+    cc,
+  },
+end
+
+/-
+  if instruction is not JMP/JMPLESS/JMPGE then it will have the next instruction just at + 1
+-/
+lemma iexec_shift_without_jmp {n : ℤ}  {i' : ℤ} {i : ℤ}:
+n + i' = n + i + 1 ↔ i' = i + 1 :=
+begin
+  apply iff.intro,
+  {
+    intro h_no_brackets,
+    have h_brackets: n + i' = n + (i + 1) := 
+    begin
+      simp [h_no_brackets],
+      cc,
+    end,
+    apply int.add_left_cancel,
+    apply h_brackets,
+  },
+  {
+    intro h3,
+    simp [h3],
+    cc,
+  },
+end
+
+
+
+lemma iexec_shift {instr n i' s' stk' i s stk}:
+((n+i',s',stk') = iexec instr (n+i, s, stk)) = ((i',s',stk') = iexec instr (i,s,stk)) :=
+begin
+  cases instr,
+  case LOADI {
+    simp [iexec],
+    intros h1 h2,
+    apply iexec_shift_without_jmp,
+  },
+  case LOAD {
+    simp [iexec],
+    intros h1 h2,
+    apply iexec_shift_without_jmp,
+
+  },
+  case ADD {
+    simp [iexec],
+    intros h1 h2,
+    apply iexec_shift_without_jmp,
+
+  },
+  case SUB {
+    simp [iexec],
+    intros h1 h2,
+    apply iexec_shift_without_jmp,
+  },
+  case MUL {
+    simp [iexec],
+    intros h1 h2,
+    apply iexec_shift_without_jmp,
+  },
+  case DIV {
+    simp [iexec],
+    intros h1 h2,
+    apply iexec_shift_without_jmp,
+  },
+  case STORE {
+    simp [iexec],
+    intros h1 h2,
+    apply iexec_shift_without_jmp,
+  },
+  case JMP {
+    simp [iexec],
+    intros h1 h2,
+    apply iexec_shift_with_jmp,
+  },
+  case JMPLESS {
+    simp [iexec],
+    cases classical.em (head2 stk < list.head stk),
+    {
+      simp [h],
+      intros h1 h2,
+      apply iexec_shift_with_jmp,
+    },
+    {
+      simp [h],
+      intros h1 h2,
+      apply iexec_shift_without_jmp,
+    }
+  },
+  case JMPGE {
+    simp [iexec],
+    cases classical.em (list.head stk ≤ head2 stk),
+    {
+      simp [h],
+      intros h1 h2,
+      apply iexec_shift_with_jmp,
+    },
+    {
+      simp [h],
+      intros h1 h2,
+      apply iexec_shift_without_jmp,
+    },
+  },
+  case NOP {
+    simp [iexec],
+    intros h1 h2,
+    apply iexec_shift_without_jmp,
+  },
+end
+
+
+
+
+
+/-
+lemma exec1_appendR: "P ⊢ c → c' ⟹ P@P' ⊢ c → c'"
+by (auto simp: exec1_def)
+-/
+lemma exec1_appendR {li c c' li'} (h: exec1 li c c'): 
+exec1 (li ++ li') c c' :=
+begin
+  -- simp [exec1],
+  -- cases c with i s_stk,
+  -- use i,
+  -- cases s_stk with s stk,
+  -- use s,
+  -- use stk,
+  -- sorry,
+  induction li with hd tl ih,
+  case list.nil {
+    sorry,
+  },
+  case list.cons {
+    rw list.cons_append,
+    sorry,
+  }
+
+
+end
+
+/-
+lemma exec_appendR: "P ⊢ c →* c' ⟹ P@P' ⊢ c →* c'"
+by (induction rule: star.induct) (fastforce intro: star.step exec1_appendR)+
+-/
+lemma exec_appendR {li c c' li'} (h: exec li c c'):
+exec (li ++ li') c c' :=
+begin
+  induction' h,
+  -- cases
+  sorry,   --TODO: what is fastforce intro?
+end
+
+/-
+lemma exec1_appendL:
+  fixes i i' :: int 
+  shows
+  "P ⊢ (i,s,stk) → (i',s',stk') ⟹
+   P' @ P ⊢ (size(P')+i,s,stk) → (size(P')+i',s',stk')"
+  unfolding exec1_def
+  by (auto simp del: iexec.simps)
+-/
+
+-- lemma exec1_appendL {i i'}  --TODO: how does fixes i i' work?
+
+/-
+lemma exec_appendL:
+  fixes i i' :: int 
+  shows
+ "P ⊢ (i,s,stk) →* (i',s',stk')  ⟹
+  P' @ P ⊢ (size(P')+i,s,stk) →* (size(P')+i',s',stk')"
+  by (induction rule: exec_induct) (blast intro: star.step exec1_appendL)+
+-/
+-- lemma exec_appendL {i i'} -- TODO: how does fixes work and what is blast intro?
+
+
+/-
+text‹Now we specialise the above lemmas to enable automatic proofs of
+\<^prop>‹P ⊢ c →* c'› where ‹P› is a mixture of concrete instructions and
+pieces of code that we already know how they execute (by induction), combined
+by ‹@› and ‹#›. Backward jumps are not supported.
+The details should be skipped on a first reading.
+
+If we have just executed the first instruction of the program, drop it:›
+
+lemma exec_Cons_1 [intro]:
+  "P ⊢ (0,s,stk) →* (j,t,stk') ⟹
+  instr#P ⊢ (1,s,stk) →* (1+j,t,stk')"
+by (drule exec_appendL[where P'="[instr]"]) simp
+
+lemma exec_appendL_if[intro]:
+  fixes i i' j :: int
+  shows
+  "size P' <= i
+   ⟹ P ⊢ (i - size P',s,stk) →* (j,s',stk')
+   ⟹ i' = size P' + j
+   ⟹ P' @ P ⊢ (i,s,stk) →* (i',s',stk')"
+by (drule exec_appendL[where P'=P']) simp
+
+text‹Split the execution of a compound program up into the execution of its
+parts:›
+
+lemma exec_append_trans[intro]:
+  fixes i' i'' j'' :: int
+  shows
+"P ⊢ (0,s,stk) →* (i',s',stk') ⟹
+ size P ≤ i' ⟹
+ P' ⊢  (i' - size P,s',stk') →* (i'',s'',stk'') ⟹
+ j'' = size P + i''
+ ⟹
+ P @ P' ⊢ (0,s,stk) →* (j'',s'',stk'')"
+by(metis star_trans[OF exec_appendR exec_appendL_if])
+
+
+declare Let_def[simp]
+
+
+subsection "Compilation"
+
+fun acomp :: "aexp ⇒ instr list" where
+"acomp (N n) = [LOADI n]" |
+"acomp (V x) = [LOAD x]" |
+"acomp (Plus a1 a2) = acomp a1 @ acomp a2 @ [ADD]"
+
+lemma acomp_correct[intro]:
+  "acomp a ⊢ (0,s,stk) →* (size(acomp a),s,aval a s#stk)"
+by (induction a arbitrary: stk) fastforce+
+
+fun bcomp :: "bexp ⇒ bool ⇒ int ⇒ instr list" where
+"bcomp (Bc v) f n = (if v=f then [JMP n] else [])" |
+"bcomp (Not b) f n = bcomp b (¬f) n" |
+"bcomp (And b1 b2) f n =
+ (let cb2 = bcomp b2 f n;
+        m = if f then size cb2 else (size cb2)+n;
+      cb1 = bcomp b1 False m
+  in cb1 @ cb2)" |
+"bcomp (Less a1 a2) f n =
+ acomp a1 @ acomp a2 @ (if f then [JMPLESS n] else [JMPGE n])"
+
+value
+  "bcomp (And (Less (V ''x'') (V ''y'')) (Not(Less (V ''u'') (V ''v''))))
+     False 3"
+
+lemma bcomp_correct[intro]:
+  fixes n :: int
+  shows
+  "0 ≤ n ⟹
+  bcomp b f n ⊢
+ (0,s,stk)  →*  (size(bcomp b f n) + (if f = bval b s then n else 0),s,stk)"
+proof(induction b arbitrary: f n)
+  case Not
+  from Not(1)[where f="~f"] Not(2) show ?case by fastforce
+next
+  case (And b1 b2)
+  from And(1)[of "if f then size(bcomp b2 f n) else size(bcomp b2 f n) + n" 
+                 "False"] 
+       And(2)[of n f] And(3) 
+  show ?case by fastforce
+qed fastforce+
+
+fun ccomp :: "com ⇒ instr list" where
+"ccomp SKIP = []" |
+"ccomp (x ::= a) = acomp a @ [STORE x]" |
+"ccomp (c⇩1;;c⇩2) = ccomp c⇩1 @ ccomp c⇩2" |
+"ccomp (IF b THEN c⇩1 ELSE c⇩2) =
+  (let cc⇩1 = ccomp c⇩1; cc⇩2 = ccomp c⇩2; cb = bcomp b False (size cc⇩1 + 1)
+   in cb @ cc⇩1 @ JMP (size cc⇩2) # cc⇩2)" |
+"ccomp (WHILE b DO c) =
+ (let cc = ccomp c; cb = bcomp b False (size cc + 1)
+  in cb @ cc @ [JMP (-(size cb + size cc + 1))])"
+
+
+value "ccomp
+ (IF Less (V ''u'') (N 1) THEN ''u'' ::= Plus (V ''u'') (N 1)
+  ELSE ''v'' ::= V ''u'')"
+
+value "ccomp (WHILE Less (V ''u'') (N 1) DO (''u'' ::= Plus (V ''u'') (N 1)))"
+
+
+subsection "Preservation of semantics"
+
+lemma ccomp_bigstep:
+  "(c,s) ⇒ t ⟹ ccomp c ⊢ (0,s,stk) →* (size(ccomp c),t,stk)"
+proof(induction arbitrary: stk rule: big_step_induct)
+  case (Assign x a s)
+  show ?case by (fastforce simp:fun_upd_def cong: if_cong)
+next
+  case (Seq c1 s1 s2 c2 s3)
+  let ?cc1 = "ccomp c1"  let ?cc2 = "ccomp c2"
+  have "?cc1 @ ?cc2 ⊢ (0,s1,stk) →* (size ?cc1,s2,stk)"
+    using Seq.IH(1) by fastforce
+  moreover
+  have "?cc1 @ ?cc2 ⊢ (size ?cc1,s2,stk) →* (size(?cc1 @ ?cc2),s3,stk)"
+    using Seq.IH(2) by fastforce
+  ultimately show ?case by simp (blast intro: star_trans)
+next
+  case (WhileTrue b s1 c s2 s3)
+  let ?cc = "ccomp c"
+  let ?cb = "bcomp b False (size ?cc + 1)"
+  let ?cw = "ccomp(WHILE b DO c)"
+  have "?cw ⊢ (0,s1,stk) →* (size ?cb,s1,stk)"
+    using ‹bval b s1› by fastforce
+  moreover
+  have "?cw ⊢ (size ?cb,s1,stk) →* (size ?cb + size ?cc,s2,stk)"
+    using WhileTrue.IH(1) by fastforce
+  moreover
+  have "?cw ⊢ (size ?cb + size ?cc,s2,stk) →* (0,s2,stk)"
+    by fastforce
+  moreover
+  have "?cw ⊢ (0,s2,stk) →* (size ?cw,s3,stk)" by(rule WhileTrue.IH(2))
+  ultimately show ?case by(blast intro: star_trans)
+qed fastforce+
+
+end
+-/
 
 
 end LoComp
